---
cssclass:
aliases:
tags:
---
**[[DISCRET12ch6|BACK]]**

---
## Example 6.2: Truth Table for p ∨ ∼q → ∼p
Construct a truth table for the statement form p ∨ ∼q → ∼p.

**Solution:**
By the order of operations given above, the following two expressions are equivalent: $p\ \ ∨ ∼q →∼p$ and $(p\ \ ∨ (∼q)) → (∼p)$, and this order governs the construction of the truth table. First fill in the four possible combinations of truth values for $p$ and $q$, and then enter the truth values for $∼p$ and $∼q$ using the definition of negation. Next fill in the $p\ \ ∨ ∼q$ column using the definition of $∨.$ Finally, fill in the $p\ \ ∨ ∼q → ∼p$ column using the definition of $→$. The only rows in which the hypothesis $p\ \ ∨ ∼q$ is true and the conclusion $∼p$ is false are the first and second rows. So you put F’s in those two rows and T’s in the other two rows.

![[DISCRET12ch6Example2image.png|center]]