---
cssclass:
aliases:
tags:
---
**[[DISCRET12ch6|BACK]]**

---
## Example 6.1: A Conditional Statement with a False Hypothesis
Consider the statement:
<center>If 0 = 1 then 1 = 2.</center>

As strange as it may seem, since the hypothesis of this statement is false, the statement
as a whole is true.

The philosopher Willard Van Orman Quine advises against using the phrase “p implies q” to mean “p → q” because the word implies suggests that q can be logically deduced from p and this is often not the case. Nonetheless, the phrase is used by many people, probably because it is a convenient replacement for the → symbol. And, of course, in many cases a conclusion can be deduced from a hypothesis, even when the hypothesis is false.

>[!NOTE|alt-co] For example,
> if $0 = 1$, then, by adding $1$ to both sides of the equation, you can deduce that $1 = 2$.

In expressions that include $→$ as well as other logical operators such as $∧,$ $∨,$ and $∼,$ the order of operations is that $→$ is performed last. Thus, according to the specification of order of operations in [[DISCRET12ch4|Section 2.1]], $∼$ is performed first, then $∧$ and $∨,$ and finally $→$.